

# Univariate Linear Regression

单变量线性回归

## 1. Form and Assumption 形式 & 假设

observation  $\{(x_i, y_i) \mid i=1, 2, \dots, n\}$

### ① Form of univariate linear regression:

$$y_i = \beta_0 + \beta_1 x_i + \varepsilon_i$$

covariance  $x_i$  is nonrandom

response  $y_i$

intercept  $\beta_0$  is unknown parameters

slope  $\beta_1$  is unknown parameters

error  $\varepsilon_i$  is random variable

误差 ( $y_i$  不能被  $x_i$  解释的部分)

### ② Assumption of $\varepsilon_i$ 只要不相关, 不需要独立

Gauss-Markov condition: for (unknown) constant  $\sigma^2$

$$E(\varepsilon_i) = 0$$

$$\text{cov}(\varepsilon_i, \varepsilon_j) = \begin{cases} 0 & i \neq j \\ \sigma^2 & i = j \end{cases}$$

### ③ Based on assumption.

$$y_i = \beta_0 + \beta_1 x_i + \varepsilon_i$$

$$E(y_i) = \beta_0 + \beta_1 x_i$$

$$\text{cov}(y_i, y_j) = \begin{cases} 0 & i \neq j \\ \sigma^2 & i = j \end{cases}$$

## 2. Estimation of the regression parameters 估计 $\beta_0, \beta_1, \sigma^2$

### ① Method 1: Ordinary least squares estimation (OLSE) 普通最小二乘法

Intuition Loss function

$$\begin{aligned} Q(\beta_0, \beta_1) &= \sum_{i=1}^n (y_i - E(y_i))^2 \\ &= \sum_{i=1}^n (y_i - \beta_0 - \beta_1 x_i)^2 \end{aligned}$$

Solution derivative of quadratic loss function

$$\left. \frac{\partial Q}{\partial \beta_0} \right|_{\beta_0 = \hat{\beta}_0} = -2 \sum_{i=1}^n (y_i - \hat{\beta}_0 - \hat{\beta}_1 x_i) = 0$$

二阶导

$$\left. \frac{\partial Q}{\partial \beta_1} \right|_{\beta_1 = \hat{\beta}_1} = -2 \sum_{i=1}^n (y_i - \hat{\beta}_0 - \hat{\beta}_1 x_i) x_i = 0$$

$$\Rightarrow \hat{\beta}_0 = \bar{y} - \bar{x} \hat{\beta}_1$$

$$\hat{\beta}_1 = \frac{\sum (x_i - \bar{x})(y_i - \bar{y})}{\sum (x_i - \bar{x})^2} = \frac{\text{cov}(x, y)}{\text{var}(x)} = \frac{L_{xy}}{L_{xx}}$$

Proof:

$$\hat{\beta}_0: \sum_{i=1}^n (y_i - \hat{\beta}_0 - \hat{\beta}_1 x_i) = 0 \Rightarrow n \hat{\beta}_0 = \sum y_i - \hat{\beta}_1 \sum x_i \Rightarrow \hat{\beta}_0 = \bar{y} - \bar{x} \hat{\beta}_1$$

$$\hat{\beta}_1: \sum_{i=1}^n (y_i - \hat{\beta}_0 - \hat{\beta}_1 x_i) x_i = 0 \Rightarrow \sum (y_i - \bar{y} + \bar{x} \hat{\beta}_1 - \hat{\beta}_1 x_i) x_i = 0$$

$$\text{LHS} = \sum x_i y_i - \bar{y} \sum x_i + \bar{x} \hat{\beta}_1 \sum x_i - \hat{\beta}_1 \sum x_i^2 = 0$$

$$\therefore \hat{\beta}_1 \sum x_i (x_i - \bar{x}) = \sum x_i (y_i - \bar{y})$$

$$\hat{\beta}_1 \sum (x_i - \bar{x} + \bar{x})(x_i - \bar{x}) = \sum (x_i - \bar{x} + \bar{x})(y_i - \bar{y})$$

$$\text{it is obvious that } \sum (x_i - \bar{x}) = \sum x_i - n\bar{x} = 0 \quad \sum (y_i - \bar{y}) = 0$$

$$\therefore \hat{\beta}_1 \sum (x_i - \bar{x})^2 = \sum (x_i - \bar{x})(y_i - \bar{y})$$

$$\Rightarrow \hat{\beta}_1 = \frac{\text{cov}(x, y)}{\text{var}(x)} = \frac{L_{xy}}{L_{xx}}$$

Remark Sum of Squares of the Residuals (Errors) 残差平方和

$$e_i = y_i - \hat{y}_i$$

$$\hat{y}_i = \hat{\beta}_0 + \hat{\beta}_1 x_i$$

$$SSE = \sum_{i=1}^n e_i^2 = \sum_{i=1}^n (y_i - \hat{\beta}_0 - \hat{\beta}_1 x_i)^2$$

Property

$$\sum_{i=1}^n e_i = 0$$

$$\sum_{i=1}^n x_i e_i = 0$$

Proof:

$$\begin{aligned}\sum e_i &= \sum (y_i - \hat{y}_i) = \sum (y_i - \hat{\beta}_0 - \hat{\beta}_1 x_i) \\&= \sum y_i - \sum (\bar{y} - \bar{x} \hat{\beta}_1) - \sum \hat{\beta}_1 x_i \\&= (\sum y_i - n\bar{y}) + n\bar{x} \hat{\beta}_1 - \hat{\beta}_1 \sum x_i \\&= \hat{\beta}_1 (n\bar{x} - \sum x_i) \\&= 0 \quad \square\end{aligned}$$

$$\begin{aligned}\sum x_i e_i &= \sum x_i (y_i - \hat{y}_i) = \sum x_i y_i - \sum x_i (\hat{\beta}_0 + \hat{\beta}_1 x_i) \\&= \sum x_i y_i - \sum x_i (\bar{y} - \bar{x} \hat{\beta}_1 + \hat{\beta}_1 x_i) \\&= \sum x_i y_i - \bar{y} \sum x_i + \bar{x} \hat{\beta}_1 \sum x_i + \hat{\beta}_1 \sum x_i^2 \\&= \sum x_i (y_i - \bar{y}) + \hat{\beta}_1 \sum x_i (\bar{x} - x_i) \\&\quad \because \hat{\beta}_1 \sum x_i (x_i - \bar{x}) = \sum x_i (y_i - \bar{y}) \\&= \sum x_i (y_i - \bar{y}) - \sum x_i (y_i - \bar{y}) \\&= 0 \quad \square\end{aligned}$$

Remark :  $\hat{\beta}_1, \hat{\beta}_2$  are random variables

while  $\beta_1, \beta_2$  are (unknown) constants

## ② Method 2: Maximum Likelihood estimation (MLE) 极大似然估计

### Add Assumption

$y_i$  are independent

i.i.d.  $\varepsilon_i \sim N(0, \sigma^2)$

therefore,  $y_i = \beta_0 + \beta_1 x_i + \varepsilon_i \sim N(\beta_0 + \beta_1 x_i, \sigma^2)$

Intuition max likelihood function (or Log-Likelihood function)

$$f_i(y_i) = \frac{1}{\sqrt{2\pi}\sigma} \cdot \exp\left\{-\frac{1}{2\sigma^2} [y_i - (\beta_0 + \beta_1 x_i)]^2\right\}$$

$$L(\beta_0, \beta_1, \sigma^2) = \prod_{i=1}^n f_i(y_i | \beta_0, \beta_1, \sigma^2)$$

$$\log(L) = -\frac{n}{2} \log(2\pi\sigma^2) - \frac{1}{2\sigma^2} \sum_{i=1}^n [y_i - (\beta_0 + \beta_1 x_i)]^2$$

### Solution

$\hat{\beta}_0, \hat{\beta}_1$  are the same

$$\left. \frac{\partial \log(L)}{\partial \sigma^2} \right|_{\sigma^2 = \hat{\sigma}^2} = -\frac{n}{2} \cdot \frac{1}{2\pi \hat{\sigma}^2} + \frac{1}{4\hat{\sigma}^4} \cdot \sum_{i=1}^n [y_i - (\hat{\beta}_0 + \hat{\beta}_1 x_i)]^2$$

$$\Rightarrow \hat{\sigma}^2 = \frac{1}{n} \sum_{i=1}^n (y_i - \hat{y}_i)^2$$

$$= \frac{1}{n} \sum_{i=1}^n (y_i - \hat{\beta}_0 - \hat{\beta}_1 x_i)^2$$

= 阶导

### Remark

$\hat{\sigma}^2 = \frac{1}{n} \sum (y_i - \hat{y}_i)^2$  is biasedness

$$\hat{\sigma}^2 = \frac{1}{n-2} \sum_{i=1}^n (y_i - \hat{y}_i)^2$$

$$= \frac{1}{n-2} \sum_{i=1}^n (y_i - \hat{\beta}_0 - \hat{\beta}_1 x_i)^2 \quad \text{is unbiasedness}$$

**Remark:** assuming  $\varepsilon_i \sim N(0, \sigma^2)$ ,  $\varepsilon_j \sim N(0, \sigma^2)$  and  $\text{cov}(\varepsilon_i, \varepsilon_j) = 0$  does **not** ensure  $\varepsilon_i \perp \varepsilon_j$ .

Property

$$\hat{\sigma}^2 = \frac{1}{n-2} \sum_{i=1}^n (y_i - \hat{y}_i)^2$$
$$= \frac{1}{n-2} \sum_{i=1}^n (y_i - \hat{\beta}_0 - \hat{\beta}_1 x_i)^2 \quad \text{is unbiasedness}$$

Proof 见 P2

### 3. Properties of Ordinary least squares estimation 最小二乘性质

★ 探究参数  $\beta_0, \beta_1$  的估计  $\hat{\beta}_0, \hat{\beta}_1$  的性质

#### ① Linearity

$\hat{\beta}_0, \hat{\beta}_1$  are linear functions of  $y_i$

$$\hat{\beta}_1 = \sum_{i=1}^n \frac{x_i - \bar{x}}{\sum_{j=1}^n (x_j - \bar{x})^2} \cdot y_i$$

$$\hat{\beta}_0 = \bar{y} - \hat{\beta}_1 \bar{x} = \sum_{i=1}^n \left\{ \frac{1}{n} - \frac{\bar{x}(x_i - \bar{x})}{\sum_{j=1}^n (x_j - \bar{x})^2} \right\} \cdot y_i$$

Proof:

$$\hat{\beta}_1 = \frac{\sum (x_i - \bar{x})(y_i - \bar{y})}{L_{xx}}$$
$$= \frac{1}{L_{xx}} \cdot \sum (x_i - \bar{x}) y_i - \frac{1}{L_{xx}} \cdot \sum (x_i - \bar{x}) \bar{y}$$
$$= \frac{1}{L_{xx}} \sum (x_i - \bar{x}) \cdot y_i - 0 \quad \square$$
$$\hat{\beta}_0 = \bar{y} - \bar{x} \hat{\beta}_1 = \frac{1}{n} \sum y_i - \frac{1}{L_{xx}} \cdot \sum \bar{x} (x_i - \bar{x}) \cdot y_i$$
$$= \sum_{i=1}^n \left\{ \frac{1}{n} - \frac{\bar{x}(x_i - \bar{x})}{\sum_{j=1}^n (x_j - \bar{x})^2} \right\} \cdot y_i \quad \square$$

#### ② Unbiasedness

$E(\hat{x}) = x$  这在实践中是有利的, 表明, 重复次数增多, 估计值的平均会越来越靠近真实值

$$E(\hat{\beta}_1) = \beta_1$$

$$E(\hat{\beta}_0) = \beta_0$$

Proof:

$$\begin{aligned} E(\hat{\beta}_1) &= \sum \frac{x_i - \bar{x}}{L_{xx}} \cdot E(y_i) \\ &= \sum \frac{x_i - \bar{x}}{L_{xx}} \cdot (\beta_0 + \beta_1 x_i) \\ &= \frac{\beta_0}{L_{xx}} \cdot \sum (x_i - \bar{x}) + \frac{\beta_1}{L_{xx}} \sum x_i (x_i - \bar{x}) \\ &= 0 + \frac{\beta_1}{L_{xx}} \sum (x_i - \bar{x} + \bar{x})(x_i - \bar{x}) \\ &= \frac{\beta_1}{L_{xx}} \cdot L_{xx} + 0 \\ &= \beta_1 \quad \square \end{aligned}$$

$$\begin{aligned} E(\hat{\beta}_0) &= E(\bar{y} - \bar{x} \hat{\beta}_1) \\ &= \frac{1}{n} \sum E(y_i) - \bar{x} \cdot E(\hat{\beta}_1) \\ &= \frac{1}{n} \cdot \sum (\beta_0 + \beta_1 x_i) - \bar{x} \cdot \beta_1 \\ &= \frac{1}{n} \cdot n\beta_0 + \beta_1 \cdot \frac{1}{n} \sum x_i - \beta_1 \bar{x} \\ &= \beta_0 \quad \square \end{aligned}$$

③ Variance and cov( $\hat{\beta}_1, \hat{\beta}_0$ )

$$\text{var}(\hat{\beta}_1) = \frac{\sigma^2}{\sum_{i=1}^n (x_i - \bar{x})^2}$$

$$\text{var}(\hat{\beta}_0) = \left[ \frac{1}{n} + \frac{\bar{x}^2}{\sum_{i=1}^n (x_i - \bar{x})^2} \right] \sigma^2$$

$$\text{cov}(\hat{\beta}_1, \hat{\beta}_0) = - \frac{\bar{x}}{\sum_{i=1}^n (x_i - \bar{x})^2} \cdot \sigma^2$$

*Proof:* 
$$\begin{aligned} \text{var}(\hat{\beta}_1) &= \text{var} \left( \sum \frac{x_i - \bar{x}}{L_{xx}} \cdot y_i \right) \\ &= \sum \left( \frac{x_i - \bar{x}}{L_{xx}} \right)^2 \cdot \text{var}(y_i) \\ &= \frac{\sum (x_i - \bar{x})^2}{L_{xx}^2} \cdot \sigma^2 \\ &= \frac{\sigma^2}{L_{xx}} \quad \square \end{aligned}$$

$$\begin{aligned} \text{var}(\hat{\beta}_0) &= \text{var}(\bar{y} - \bar{x} \hat{\beta}_1) \\ &= \text{var}(\bar{y}) + \text{var}(\bar{x} \hat{\beta}_1) + 0 \\ &= \left( \frac{1}{n} \sum \text{var}(y_i) + 0 + 0 + \dots + 0 \right) + \bar{x}^2 \cdot \frac{\sigma^2}{L_{xx}} \\ &= \frac{1}{n} \cdot \sigma^2 + \bar{x}^2 \cdot \frac{\sigma^2}{L_{xx}} \\ &= \left( \frac{1}{n} + \frac{\bar{x}^2}{L_{xx}} \right) \sigma^2 \quad \square \end{aligned}$$

$$\begin{aligned} \text{cov}(\hat{\beta}_1, \hat{\beta}_0) &= E(\hat{\beta}_1 - E(\hat{\beta}_1))(\hat{\beta}_0 - E(\hat{\beta}_0)) \\ &= E(\hat{\beta}_1 - \beta_1)(\hat{\beta}_0 - \beta_0) \\ &= E(\hat{\beta}_1 - \beta_1)(\bar{y} - \bar{x} \hat{\beta}_1 - \beta_0) \\ &= E[(\hat{\beta}_1 - \beta_1)\bar{y}] - E[(\hat{\beta}_1 - \beta_1)\bar{x}\hat{\beta}_1] - E[(\hat{\beta}_1 - \beta_1)\beta_0] \\ &\because E(\hat{\beta}_1 - \beta_1) = E(\hat{\beta}_1) - \beta_1 = 0 \end{aligned}$$

$$\begin{aligned} \bar{y} &= \frac{1}{n} \sum (\beta_0 + \beta_1 x_i) \quad \beta_0, \beta_1, x_i \in \text{const} \\ &= 0 - \bar{x} E(\hat{\beta}_1^2 - \beta_1 \hat{\beta}_1) - 0 \\ &= -\bar{x} E(\hat{\beta}_1^2) + \bar{x} \beta_1 E(\hat{\beta}_1) \\ &= -\bar{x} [\text{var}(\hat{\beta}_1) + (E(\hat{\beta}_1))^2] + \bar{x} \beta_1^2 \\ &= -\bar{x} \cdot \frac{\sigma^2}{L_{xx}} - \bar{x} \beta_1^2 + \bar{x} \beta_1^2 \\ &= -\frac{\bar{x}}{L_{xx}} \cdot \sigma^2 \quad \square \end{aligned}$$

$$\begin{aligned} \hat{\beta}_1 &= \sum_{i=1}^n \frac{x_i - \bar{x}}{\sum_{j=1}^n (x_j - \bar{x})^2} \cdot y_i \\ \hat{\beta}_0 &= \bar{y} - \hat{\beta}_1 \bar{x} = \sum_{i=1}^n \left\{ \frac{1}{n} - \frac{\bar{x}(x_i - \bar{x})}{\sum_{j=1}^n (x_j - \bar{x})^2} \right\} \cdot y_i \end{aligned} \quad \left. \vphantom{\sum_{i=1}^n} \right\} \text{cov}(\hat{\beta}_1, \hat{\beta}_0)$$

#### ④ Distribution

##### Add Assumption

$$① \varepsilon_i \sim N(0, \sigma^2)$$

$$② y_i \sim N(\beta_0 + \beta_1 x_i, \sigma^2), \quad y_i \text{ independent}$$

$\therefore$  Linearity

$$\hat{\beta}_1 \sim N\left(\beta_1, \frac{\sigma^2}{\sum_{i=1}^n (x_i - \bar{x})^2}\right)$$

$$\hat{\beta}_0 \sim N\left(\beta_0, \left[\frac{1}{n} + \frac{\bar{x}^2}{\sum_{i=1}^n (x_i - \bar{x})^2}\right] \sigma^2\right)$$

#### ⑤ MLE Assume $\varepsilon_i \sim N(0, \sigma^2)$

残差  $e_i = y_i - \hat{y}_i$  与  $\hat{\beta}_1, \hat{\beta}_0$  不相关 (不代表独立)

$$\text{cov}(e_i, \hat{\beta}_1) = 0$$

$$\text{cov}(e_i, \hat{\beta}_0) = 0$$

Proof:

$$\begin{aligned} \text{cov}(e_i, \hat{\beta}_0) &= \text{cov}(y_i - \hat{\beta}_0 - \hat{\beta}_1 x_i, \hat{\beta}_0) \\ &= \text{cov}(y_i, \hat{\beta}_0) - \text{var}(\hat{\beta}_0) - x_i \cdot \text{cov}(\hat{\beta}_1, \hat{\beta}_0) \end{aligned}$$

$$\begin{aligned} \therefore \hat{\beta}_0 &= \sum \left(\frac{1}{n} - \frac{\bar{x}(x_i - \bar{x})}{L_{xx}}\right) \cdot y_i \quad \text{cov}(y_i, y_j) = 0 \quad i \neq j \\ \therefore &= \left(\frac{1}{n} - \frac{\bar{x}(x_i - \bar{x})}{L_{xx}}\right) \cdot \sigma^2 - \left(\frac{1}{n} + \frac{\bar{x}^2}{L_{xx}}\right) \sigma^2 + x_i \cdot \frac{\bar{x}}{L_{xx}} \cdot \sigma^2 \\ &= 0 \quad \square \end{aligned}$$

$$\begin{aligned} \text{cov}(e_i, \hat{\beta}_1) &= \text{cov}(y_i - \hat{\beta}_0 - \hat{\beta}_1 x_i, \hat{\beta}_1) \\ &= \text{cov}(y_i, \hat{\beta}_1) - \text{cov}(\hat{\beta}_0, \hat{\beta}_1) - x_i \cdot \text{var}(\hat{\beta}_1) \end{aligned}$$

$$\begin{aligned} \therefore \hat{\beta}_1 &= \sum \frac{x_i - \bar{x}}{L_{xx}} y_i \quad \text{cov}(y_i, y_j) = 0 \quad i \neq j \\ &= \frac{x_i - \bar{x}}{L_{xx}} \sigma^2 + \frac{\bar{x}}{L_{xx}} \sigma^2 - x_i \cdot \frac{\sigma^2}{L_{xx}} \end{aligned}$$



$$= 0 \quad \square$$

⑥ MLE,  $\hat{\sigma}^2$  的无偏估计 见 1.2

\*

$$\begin{aligned}\hat{\sigma}^2 &= \frac{1}{n-2} \sum_{i=1}^n (y_i - \hat{y}_i)^2 \\ &= \frac{1}{n-2} \sum_{i=1}^n (y_i - \hat{\beta}_0 - \hat{\beta}_1 x_i)^2 \quad \text{is unbiasedness}\end{aligned}$$

Rm.  $y_i, \hat{\beta}_0, \hat{\beta}_1$  是随机变量,  $\beta_0, \beta_1, x_i$  为定常数

Proof  $e_i = y_i - \hat{y}_i = y_i - \hat{\beta}_0 - \hat{\beta}_1 x_i$

$$E(\sum e_i^2) = E(\sum (y_i - \hat{y}_i)^2) = \sum \underbrace{E(y_i - \hat{y}_i)^2}_{①}$$

$$① = [E(y_i - \hat{y}_i)]^2 + \underbrace{\text{var}(y_i - \hat{y}_i)}_{③}$$

$$② = E(y_i) - E(\hat{y}_i) = \beta_0 + \beta_1 x_i - \beta_0 - \beta_1 x_i = 0$$

$$\begin{aligned}③ &= \text{var}(y_i) + \text{var}(\hat{y}_i) - 2 \text{cov}(y_i, \hat{y}_i) \\ &= \sigma^2 + \underbrace{\text{var}(\hat{\beta}_0 + \hat{\beta}_1 x_i)}_{④} - 2 \underbrace{\text{cov}(y_i, \hat{\beta}_0 + \hat{\beta}_1 x_i)}_{⑤}\end{aligned}$$

$$④ = \text{var}(\hat{\beta}_0) + x_i^2 \cdot \text{var}(\hat{\beta}_1) + 2x_i \text{cov}(\hat{\beta}_0, \hat{\beta}_1)$$

$$= \left(\frac{1}{n} + \frac{\bar{x}^2}{L_{xx}}\right) \sigma^2 + x_i^2 \cdot \frac{1}{L_{xx}} \sigma^2 - 2x_i \frac{\bar{x}}{L_{xx}} \sigma^2$$

$$= \frac{\sigma^2}{n} + \frac{\sigma^2}{L_{xx}} (\bar{x}^2 + x_i^2 - 2\bar{x}x_i)$$

$$= \frac{\sigma^2}{n} + \frac{\sigma^2}{L_{xx}} (x_i - \bar{x})^2$$

$$⑤ = \text{cov}(y_i, \hat{\beta}_0) + x_i \cdot \text{cov}(y_i, \hat{\beta}_1)$$

$$\text{cov}(y_i, \hat{\beta}_0) = \left(\frac{1}{n} - \frac{\bar{x}(x_i - \bar{x})}{L_{xx}}\right) \cdot \sigma^2$$

$$\text{cov}(y_i, \hat{\beta}_1) = \frac{x_i - \bar{x}}{L_{xx}} \sigma^2$$

$$= \frac{\sigma^2}{n} - \frac{\bar{x}(x_i - \bar{x})}{L_{xx}} \sigma^2 + \frac{x_i(x_i - \bar{x})}{L_{xx}} \sigma^2$$

$$= \frac{\sigma^2}{n} + \frac{\sigma^2}{L_{xx}} (x_i - \bar{x}) \cdot (x_i - \bar{x}) = \frac{\sigma^2}{n} + \frac{(x_i - \bar{x})^2}{L_{xx}} \sigma^2$$

$$\begin{aligned} \therefore \textcircled{1} &= E(y_i - \hat{y}_i)^2 \\ &= \sigma^2 + \frac{\sigma^2}{n} + \frac{\sigma^2}{L_{xx}} (x_i - \bar{x})^2 - 2 \left( \frac{\sigma^2}{n} + \frac{(x_i - \bar{x})^2}{L_{xx}} \sigma^2 \right) \\ &= \sigma^2 \left( 1 + \frac{1}{n} + \frac{1}{L_{xx}} (x_i - \bar{x})^2 - \frac{2}{n} - \frac{2}{L_{xx}} (x_i - \bar{x})^2 \right) \\ &= \sigma^2 \left( 1 - \frac{1}{n} - \frac{1}{L_{xx}} (x_i - \bar{x})^2 \right) \end{aligned}$$

$$\begin{aligned} \therefore E(\hat{\sigma}^2) &= \frac{1}{n-2} \sum E(e_i^2) \\ &= \frac{1}{n-2} \sum \sigma^2 \left( 1 - \frac{1}{n} - \frac{(x_i - \bar{x})^2}{L_{xx}} \right) \\ &= \frac{1}{n-2} \left( n - 1 - \sum \frac{(x_i - \bar{x})^2}{L_{xx}} \right) \sigma^2 \\ &= \frac{1}{n-2} (n - 1 - 1) \sigma^2 \\ &= \sigma^2 \quad \square \end{aligned}$$

⑦. 对于固定的  $i$ ,  $\hat{y}_i$  也是  $y_1, \dots, y_n$  的线性组合

$$\hat{y}_i = \hat{\beta}_0 + \hat{\beta}_1 x_i$$

$$\hat{y}_i \sim N(\beta_0 + \beta_1 x_i, \left( \frac{1}{n} + \frac{(x_i - \bar{x})^2}{L_{xx}} \right) \sigma^2)$$

Remark:  $x_i$  固定 ( $i$  固定)

Proof:

$$\textcircled{1} E(\hat{y}_i) = E(\hat{\beta}_0) + E(\hat{\beta}_1) x_i = \beta_0 + \beta_1 x_i \quad \square$$

$$\begin{aligned} \textcircled{2} \text{Var}(\hat{y}_i) &= \text{Var}(\hat{\beta}_0 + \hat{\beta}_1 x_i) \\ &= \text{Var}(\hat{\beta}_0) + \text{Var}(\hat{\beta}_1 x_i) + 2 \text{cov}(\hat{\beta}_0, \hat{\beta}_1 x_i) \\ &= \left( \frac{1}{n} + \frac{\bar{x}^2}{L_{xx}} \right) \sigma^2 + x_i^2 \cdot \frac{\sigma^2}{L_{xx}} - 2 x_i \cdot \frac{\bar{x}}{L_{xx}} \sigma^2 \\ &= \left( \frac{1}{n} + \frac{(x_i - \bar{x})^2}{L_{xx}} \right) \sigma^2 \quad \square \end{aligned}$$